vale/code/arch/x64/interop/Vale.AsLowStar.LowStarSig.fst
@@ -3,7 +3,8 @@ open X64.MemoryAdapters
 open Interop.Base
 module B = LowStar.Buffer
 module BS = X64.Bytes_Semantics_s
-module BV = LowStar.BufferView
+module UV = LowStar.BufferView.Up
+module DV = LowStar.BufferView.Down
 module HS = FStar.HyperStack
 module ME = X64.Memory
 module TS = X64.Taint_Semantics_s
@@ -52,14 +53,14 @@ let uint_to_nat_seq_t
 
 [@__reduce__]
 let view_of_base_typ (t:ME.base_typ)
-  : BV.view UInt8.t (base_typ_as_type t)
+  : UV.view UInt8.t (base_typ_as_type t)
   = let open ME in
     match t with
-    | TUInt8 -> Views.view8
-    | TUInt16 -> Views.view16
-    | TUInt32 -> Views.view32
-    | TUInt64 -> Views.view64
-    | TUInt128 -> Views.view128
+    | TUInt8 -> Views.up_view8
+    | TUInt16 -> Views.up_view16
+    | TUInt32 -> Views.up_view32
+    | TUInt64 -> Views.up_view64
+    | TUInt128 -> Views.up_view128
 
 //////////////////////////////////////////////////////////////////////////////////////////
 //lowstar_sig pre post:
@@ -71,25 +72,29 @@ module IB = Interop.Base
 
 [@__reduce__]
 let mem_correspondence_1
-      (t:ME.base_typ)
-      (x:IB.buf_t t)
+      (src t:ME.base_typ)
+      (x:IB.buf_t src t)
       (h:HS.mem)
       (s:VS.state) =
   let y = as_vale_buffer x in
+  let db = get_downview x in
+  DV.length_eq db;
   Seq.equal
     (nat_to_uint_seq_t t (ME.buffer_as_seq s.VS.mem y))
-    (BV.as_seq h (BV.mk_buffer_view x (view_of_base_typ t)))
+    (UV.as_seq h (UV.mk_buffer db (view_of_base_typ t)))
 
 [@__reduce__]
 let mem_imm_correspondence_1
-      (t:ME.base_typ)
-      (x:IB.ibuf_t t)
+      (src t:ME.base_typ)
+      (x:IB.ibuf_t src t)
       (h:HS.mem)
       (s:VS.state) =
   let y = as_vale_immbuffer x in
+  let db = get_downview x in
+  DV.length_eq db;
   Seq.equal
     (nat_to_uint_seq_t t (ME.buffer_as_seq s.VS.mem y))
-    (BV.as_seq h (BV.mk_buffer_view x (view_of_base_typ t)))
+    (UV.as_seq h (UV.mk_buffer db (view_of_base_typ t)))
 
 [@__reduce__]
 let rec mem_correspondence (args:list arg) : hsprop =
@@ -98,13 +103,13 @@ let rec mem_correspondence (args:list arg) : hsprop =
   | hd :: tl ->
     let (| tag, x |) = hd in
     match tag with
-    | TD_Buffer bt _ ->
+    | TD_Buffer src bt _ ->
       fun h s ->
-        mem_correspondence_1 bt x h s /\
+        mem_correspondence_1 src bt x h s /\
         mem_correspondence tl h s
-    | TD_ImmBuffer bt _ ->
+    | TD_ImmBuffer src bt _ ->
       fun h s ->
-        mem_imm_correspondence_1 bt x h s /\
+        mem_imm_correspondence_1 src bt x h s /\
         mem_correspondence tl h s        
     | TD_Base _ ->
       mem_correspondence tl
@@ -122,12 +127,12 @@ let arg_as_nat64 (a:arg) (s:VS.state) : GTot ME.nat64 =
      UInt32.v x
   | TD_Base TUInt64 ->
      UInt64.v x
-  | TD_Buffer bt _ ->
-     buffer_addr_is_nat64 (as_vale_buffer #bt x) s;
-     ME.buffer_addr (as_vale_buffer #bt x) VS.(s.mem)
-  | TD_ImmBuffer bt _ ->
-     buffer_addr_is_nat64 (as_vale_immbuffer #bt x) s;
-     ME.buffer_addr (as_vale_immbuffer #bt x) VS.(s.mem)
+  | TD_Buffer src bt _ ->
+     buffer_addr_is_nat64 (as_vale_buffer #src #bt x) s;
+     ME.buffer_addr (as_vale_buffer #src #bt x) VS.(s.mem)
+  | TD_ImmBuffer src bt _ ->
+     buffer_addr_is_nat64 (as_vale_immbuffer #src #bt x) s;
+     ME.buffer_addr (as_vale_immbuffer #src #bt x) VS.(s.mem)
     
 
 [@__reduce__]
@@ -146,27 +151,27 @@ let rec register_args (max_arity:nat)
 let taint_hyp_arg (m:ME.mem) (tm:MS.memTaint_t) (a:arg) =
    let (| tag, x |) = a in
     match tag with
-    | TD_Buffer TUInt64 {taint=tnt} ->
+    | TD_Buffer src TUInt64 {taint=tnt} ->
       ME.valid_taint_buf64
-         (as_vale_buffer #TUInt64 x)
+         (as_vale_buffer #src #TUInt64 x)
          m
          tm
          tnt
-    | TD_Buffer TUInt128 {taint=tnt} ->
+    | TD_Buffer src TUInt128 {taint=tnt} ->
       ME.valid_taint_buf128
-         (as_vale_buffer #TUInt128 x)
+         (as_vale_buffer #src #TUInt128 x)
          m
          tm
          tnt
-    | TD_ImmBuffer TUInt64 {taint=tnt} ->
+    | TD_ImmBuffer src TUInt64 {taint=tnt} ->
       ME.valid_taint_buf64
-         (as_vale_immbuffer #TUInt64 x)
+         (as_vale_immbuffer #src #TUInt64 x)
          m
          tm
          tnt
-    | TD_ImmBuffer TUInt128 {taint=tnt} ->
+    | TD_ImmBuffer src TUInt128 {taint=tnt} ->
       ME.valid_taint_buf128
-         (as_vale_immbuffer #TUInt128 x)
+         (as_vale_immbuffer #src #TUInt128 x)
          m
          tm
          tnt         
