vale/code/arch/x64/interop/Vale.AsLowStar.MemoryHelpers.fsti
@@ -3,7 +3,8 @@ open X64.MemoryAdapters
 open Interop.Base
 module B = LowStar.Buffer
 module BS = X64.Bytes_Semantics_s
-module BV = LowStar.BufferView
+module DV = LowStar.BufferView.Down
+module UV = LowStar.BufferView.Up
 module HS = FStar.HyperStack
 module ME = X64.Memory
 module MES = X64.Memory_Sems
@@ -21,12 +22,12 @@ module ST = FStar.HyperStack.ST
 module I = Interop
 open FStar.Mul
 
-val as_vale_buffer_len (#t:base_typ) (x:buf_t t)
-   : Lemma (V.buffer_length (as_vale_buffer x) == B.length x / view_n t)
+val as_vale_buffer_len (#src #t:base_typ) (x:buf_t src t)
+   : Lemma (V.buffer_length (as_vale_buffer x) == (B.length x * view_n src) / view_n t)
            [SMTPat (V.buffer_length (as_vale_buffer x))]
 
-val as_vale_immbuffer_len (#t:base_typ) (x:ibuf_t t)
-   : Lemma (V.buffer_length (as_vale_immbuffer x) == B.length x / view_n t)
+val as_vale_immbuffer_len (#src #t:base_typ) (x:ibuf_t src t)
+   : Lemma (V.buffer_length (as_vale_immbuffer x) == (B.length x * view_n src) / view_n t)
            [SMTPat (V.buffer_length (as_vale_immbuffer x))]
 
 val state_eq_down_mem (va_s1:V.va_state) (s1:_)
@@ -46,38 +47,37 @@ val relate_modifies (args:list arg) (m0 m1 : ME.mem)
                    (hs_of_mem (as_mem m0))
                    (hs_of_mem (as_mem m1)))
 
-val reveal_readable (#t:_) (x:buf_t t) (s:ME.mem)
+val reveal_readable (#src #t:_) (x:buf_t src t) (s:ME.mem)
   : Lemma 
-      ( List.memP (Buffer x true) (ptrs_of_mem (as_mem s)) <==>
+      ( List.memP (mut_to_b8 src x) (ptrs_of_mem (as_mem s)) <==>
         ME.buffer_readable s (as_vale_buffer x) )
 
-val reveal_imm_readable (#t:_) (x:ibuf_t t) (s:ME.mem)
+val reveal_imm_readable (#src #t:_) (x:ibuf_t src t) (s:ME.mem)
   : Lemma 
-      ( List.memP (imm_to_b8 x) (ptrs_of_mem (as_mem s)) <==>
+      ( List.memP (imm_to_b8 src x) (ptrs_of_mem (as_mem s)) <==>
         ME.buffer_readable s (as_vale_immbuffer x) )
 
-val readable_live (#t:_) (x:buf_t t) (s:ME.mem)
+val readable_live (#src #t:_) (x:buf_t src t) (s:ME.mem)
   : Lemma 
       ( ME.buffer_readable s (as_vale_buffer x) ==>
         B.live (hs_of_mem (as_mem s)) x)
 
-val readable_imm_live (#t:_) (x:ibuf_t t) (s:ME.mem)
+val readable_imm_live (#src #t:_) (x:ibuf_t src t) (s:ME.mem)
   : Lemma 
       ( ME.buffer_readable s (as_vale_immbuffer x) ==>
         B.live (hs_of_mem (as_mem s)) x)
 
-
 val buffer_readable_reveal 
   (#max_arity:_)
   (#n:_)
-  (bt:base_typ)
-  (x:buf_t bt)
+  (src bt:base_typ)
+  (x:buf_t src bt)
   (args:IX64.arity_ok max_arity arg)
   (h0:HS.mem)
   (stack:IX64.stack_buffer n{mem_roots_p h0 (arg_of_sb stack::args)}) : Lemma (
     let mem = mk_mem (arg_of_sb stack::args) h0 in
-    ME.buffer_readable (as_vale_mem mem) (as_vale_buffer #bt x) <==>
-      List.memP (Buffer x true) (ptrs_of_mem mem))
+    ME.buffer_readable (as_vale_mem mem) (as_vale_buffer x) <==>
+      List.memP (mut_to_b8 src x) (ptrs_of_mem mem))
 
 val get_heap_mk_mem_reveal
   (#max_arity:_)
@@ -92,66 +92,74 @@ val get_heap_mk_mem_reveal
 val buffer_as_seq_reveal
   (#max_arity:_)
   (#n:_)
-  (t:ME.base_typ)
-  (x:buf_t t)
+  (src t:ME.base_typ)
+  (x:buf_t src t)
   (args:IX64.arity_ok max_arity arg)
   (h0:HS.mem)
   (stack:IX64.stack_buffer n{mem_roots_p h0 (arg_of_sb stack::args)}) : Lemma
   (let y = as_vale_buffer x in
+   let db = get_downview x in
+   DV.length_eq db;
    let mem = mk_mem (arg_of_sb stack::args) h0 in
    Seq.equal 
     (LSig.nat_to_uint_seq_t t (ME.buffer_as_seq (as_vale_mem mem) y))
-    (BV.as_seq h0 (BV.mk_buffer_view x (LSig.view_of_base_typ t))))
+    (UV.as_seq h0 (UV.mk_buffer db (LSig.view_of_base_typ t))))
 
 val immbuffer_as_seq_reveal
   (#max_arity:_)
   (#n:_)
-  (t:ME.base_typ)
-  (x:ibuf_t t)
+  (src t:ME.base_typ)
+  (x:ibuf_t src t)
   (args:IX64.arity_ok max_arity arg)
   (h0:HS.mem)
   (stack:IX64.stack_buffer n{mem_roots_p h0 (arg_of_sb stack::args)}) : Lemma
   (let y = as_vale_immbuffer x in
+   let db = get_downview x in
+   DV.length_eq db;
    let mem = mk_mem (arg_of_sb stack::args) h0 in
    Seq.equal 
     (LSig.nat_to_uint_seq_t t (ME.buffer_as_seq (as_vale_mem mem) y))
-    (BV.as_seq h0 (BV.mk_buffer_view x (LSig.view_of_base_typ t))))
+    (UV.as_seq h0 (UV.mk_buffer db (LSig.view_of_base_typ t))))
 
 val buffer_as_seq_reveal2
-  (t:ME.base_typ)
-  (x:buf_t t)
+  (src t:ME.base_typ)
+  (x:buf_t src t)
   (va_s:V.va_state) : Lemma
   (let y = as_vale_buffer x in
+   let db = get_downview x in
+   DV.length_eq db;
    let h = hs_of_mem (as_mem va_s.VS.mem) in
    Seq.equal 
     (LSig.nat_to_uint_seq_t t (ME.buffer_as_seq va_s.VS.mem y))
-    (BV.as_seq h (BV.mk_buffer_view x (LSig.view_of_base_typ t))))
+    (UV.as_seq h (UV.mk_buffer db (LSig.view_of_base_typ t))))
 
 val immbuffer_as_seq_reveal2
-  (t:ME.base_typ)
-  (x:ibuf_t t)
+  (src t:ME.base_typ)
+  (x:ibuf_t src t)
   (va_s:V.va_state) : Lemma
   (let y = as_vale_immbuffer x in
+   let db = get_downview x in
+   DV.length_eq db;
    let h = hs_of_mem (as_mem va_s.VS.mem) in
    Seq.equal 
     (LSig.nat_to_uint_seq_t t (ME.buffer_as_seq va_s.VS.mem y))
-    (BV.as_seq h (BV.mk_buffer_view x (LSig.view_of_base_typ t))))
+    (UV.as_seq h (UV.mk_buffer db (LSig.view_of_base_typ t))))
 
 val buffer_addr_reveal
-  (t:ME.base_typ)
-  (x:buf_t t)
+  (src t:ME.base_typ)
+  (x:buf_t src t)
   (args:list arg)
   (h0:HS.mem{mem_roots_p h0 args}) : Lemma
   (let mem = mk_mem args h0 in
-   addrs_of_mem mem (Buffer x true) == ME.buffer_addr (as_vale_buffer #t x) (as_vale_mem mem))
+   addrs_of_mem mem (mut_to_b8 src x) == ME.buffer_addr (as_vale_buffer x) (as_vale_mem mem))
 
 val immbuffer_addr_reveal
-  (t:ME.base_typ)
-  (x:ibuf_t t)
+  (src t:ME.base_typ)
+  (x:ibuf_t src t)
   (args:list arg)
   (h0:HS.mem{mem_roots_p h0 args}) : Lemma
   (let mem = mk_mem args h0 in
-   addrs_of_mem mem (imm_to_b8 x) == ME.buffer_addr (as_vale_immbuffer #t x) (as_vale_mem mem))
+   addrs_of_mem mem (imm_to_b8 src x) == ME.buffer_addr (as_vale_immbuffer x) (as_vale_mem mem))
 
 val fuel_eq : squash (V.va_fuel == nat)
 
@@ -162,18 +170,17 @@ val decls_eval_code_reveal
   (requires (V.eval_code c va_s0 f va_s1))
   (ensures (VL.eval_code c va_s0 (coerce f) va_s1))
 
-val as_vale_buffer_disjoint (#t1 #t2:base_typ) (x:buf_t t1) (y:buf_t t2)
+val as_vale_buffer_disjoint (#src1 #src2 #t1 #t2:base_typ) (x:buf_t src1 t1) (y:buf_t src2 t2)
    : Lemma (B.disjoint x y ==> ME.loc_disjoint (ME.loc_buffer (as_vale_buffer x)) (ME.loc_buffer (as_vale_buffer y)))
            [SMTPat (ME.loc_disjoint (ME.loc_buffer (as_vale_buffer x)) (ME.loc_buffer (as_vale_buffer y)))]
 
-val as_vale_buffer_imm_disjoint (#t1 #t2:base_typ) (x:ibuf_t t1) (y:buf_t t2)
+val as_vale_buffer_imm_disjoint (#src1 #src2 #t1 #t2:base_typ) (x:ibuf_t src1 t1) (y:buf_t src2 t2)
    : Lemma (B.disjoint x y ==> ME.loc_disjoint (ME.loc_buffer (as_vale_immbuffer x)) (ME.loc_buffer (as_vale_buffer y)))
            [SMTPat (ME.loc_disjoint (ME.loc_buffer (as_vale_immbuffer x)) (ME.loc_buffer (as_vale_buffer y)))]
 
-val as_vale_immbuffer_imm_disjoint (#t1 #t2:base_typ) (x:ibuf_t t1) (y:ibuf_t t2)
+val as_vale_immbuffer_imm_disjoint (#src1 #src2 #t1 #t2:base_typ) (x:ibuf_t src1 t1) (y:ibuf_t src2 t2)
    : Lemma (B.disjoint x y ==> ME.loc_disjoint (ME.loc_buffer (as_vale_immbuffer x)) (ME.loc_buffer (as_vale_immbuffer y)))
            [SMTPat (ME.loc_disjoint (ME.loc_buffer (as_vale_immbuffer x)) (ME.loc_buffer (as_vale_immbuffer y)))]
-
 
 val modifies_same_roots
   (s:ME.loc)
@@ -203,52 +210,59 @@ val core_create_lemma_taint_hyp
                 LSig.taint_hyp args va_s /\
                 ME.valid_taint_buf64 (as_vale_buffer stack) va_s.VS.mem va_s.VS.memTaint X64.Machine_s.Public))
 
-val buffer_writeable_reveal (t:ME.base_typ) (x:buf_t t) : Lemma
+val buffer_writeable_reveal (src t:ME.base_typ) (x:buf_t src t) : Lemma
   (ME.buffer_writeable (as_vale_buffer x))
 
-let low_buffer_read (t:base_typ) (h:HS.mem) (b:(buf_t t){B.live h b}) (i:nat{i < B.length b / view_n t}) : GTot (base_typ_as_type t) =
+let low_buffer_read (src t:base_typ) (h:HS.mem) (b:(buf_t src t){B.live h b}) (i:nat{i < DV.length (get_downview b) / view_n t}) : GTot (base_typ_as_type t) =
   let view = LSig.view_of_base_typ t in
-  let b_v = BV.mk_buffer_view b view in
-  BV.as_buffer_mk_buffer_view b view;
-  BV.get_view_mk_buffer_view b view;
-  BV.length_eq b_v;  
-  BV.sel h b_v i
+  let db = get_downview b in
+  DV.length_eq db;
+  let b_v = UV.mk_buffer db view in
+  UV.length_eq b_v;  
+  UV.sel h b_v i
 
-val buffer_read_reveal (t:base_typ) (h:HS.mem) (s:ME.mem) (b:(buf_t t){B.live h b}) (i:nat{i < B.length b / view_n t}) : Lemma
-  (requires Seq.equal 
+val buffer_read_reveal (src t:base_typ) (h:HS.mem) (s:ME.mem) (b:(buf_t src t){B.live h b}) (i:nat{i < DV.length (get_downview b) / view_n t}) : Lemma
+  (requires (
+   DV.length_eq (get_downview b);
+   Seq.equal 
     (LSig.nat_to_uint_seq_t t (ME.buffer_as_seq s (as_vale_buffer b)))
-    (BV.as_seq h (BV.mk_buffer_view b (LSig.view_of_base_typ t))))
+    (UV.as_seq h (UV.mk_buffer (get_downview b) (LSig.view_of_base_typ t)))))
   (ensures LSig.nat_to_uint t (ME.buffer_read (as_vale_buffer b) i s) == 
-    low_buffer_read t h b i ) 
-  [SMTPat (low_buffer_read t h b i); SMTPat (ME.buffer_read (as_vale_buffer b) i s)]
+    low_buffer_read src t h b i ) 
+  [SMTPat (low_buffer_read src t h b i); SMTPat (ME.buffer_read (as_vale_buffer b) i s)]
 
-let imm_low_buffer_read (t:base_typ) (h:HS.mem) (b:(ibuf_t t){B.live h b}) (i:nat{i < B.length b / view_n t}) : GTot (base_typ_as_type t) =
+let imm_low_buffer_read (src t:base_typ) (h:HS.mem) (b:(ibuf_t src t){B.live h b}) (i:nat{i < DV.length (get_downview b) / view_n t}) : GTot (base_typ_as_type t) =
   let view = LSig.view_of_base_typ t in
-  let b_v = BV.mk_buffer_view b view in
-  BV.as_buffer_mk_buffer_view b view;
-  BV.get_view_mk_buffer_view b view;
-  BV.length_eq b_v;  
-  BV.sel h b_v i
+  let db = get_downview b in
+  DV.length_eq db;
+  let b_v = UV.mk_buffer db view in
+  UV.length_eq b_v;  
+  UV.sel h b_v i
 
-val imm_buffer_read_reveal (t:base_typ) (h:HS.mem) (s:ME.mem) (b:(ibuf_t t){B.live h b}) (i:nat{i < B.length b / view_n t}) : Lemma
-  (requires Seq.equal 
+val imm_buffer_read_reveal (src t:base_typ) (h:HS.mem) (s:ME.mem) (b:(ibuf_t src t){B.live h b}) (i:nat{i < DV.length (get_downview b) / view_n t}) : Lemma
+  (requires (
+  DV.length_eq (get_downview b);
+  Seq.equal 
     (LSig.nat_to_uint_seq_t t (ME.buffer_as_seq s (as_vale_immbuffer b)))
-    (BV.as_seq h (BV.mk_buffer_view b (LSig.view_of_base_typ t))))
+    (UV.as_seq h (UV.mk_buffer (get_downview b) (LSig.view_of_base_typ t)))))
   (ensures LSig.nat_to_uint t (ME.buffer_read (as_vale_immbuffer b) i s) == 
-    imm_low_buffer_read t h b i ) 
-  [SMTPat (imm_low_buffer_read t h b i); SMTPat (ME.buffer_read (as_vale_immbuffer b) i s)]
+    imm_low_buffer_read src t h b i ) 
+  [SMTPat (imm_low_buffer_read src t h b i); SMTPat (ME.buffer_read (as_vale_immbuffer b) i s)]
 
-val buffer_as_seq_invert (t:base_typ) (h:HS.mem) (s:ME.mem) (b:(buf_t t){B.live h b}) : Lemma
-  (requires Seq.equal 
+val buffer_as_seq_invert (src t:base_typ) (h:HS.mem) (s:ME.mem) (b:(buf_t src t){B.live h b}) : Lemma
+  (requires (
+  DV.length_eq (get_downview b);
+  Seq.equal 
     (LSig.nat_to_uint_seq_t t (ME.buffer_as_seq s (as_vale_buffer b)))
-    (BV.as_seq h (BV.mk_buffer_view b (LSig.view_of_base_typ t))))
+    (UV.as_seq h (UV.mk_buffer (get_downview b) (LSig.view_of_base_typ t)))))
   (ensures ME.buffer_as_seq s (as_vale_buffer b) == 
-    (LSig.uint_to_nat_seq_t t (BV.as_seq h (BV.mk_buffer_view b (LSig.view_of_base_typ t)))))
-  [SMTPat (BV.as_seq h (BV.mk_buffer_view b (LSig.view_of_base_typ t)));
+    (LSig.uint_to_nat_seq_t t (UV.as_seq h (UV.mk_buffer (get_downview b) (LSig.view_of_base_typ t)))))
+  [SMTPat (UV.as_seq h (UV.mk_buffer (get_downview b) (LSig.view_of_base_typ t)));
    SMTPat (ME.buffer_as_seq s (as_vale_buffer b))]
 
 val buffer_as_seq_reveal_tuint128
-  (x:buf_t TUInt128)
+  (src:base_typ)
+  (x:buf_t src TUInt128)
   (va_s:V.va_state) : Lemma
   (let y = as_vale_buffer x in
    let h = hs_of_mem (as_mem va_s.VS.mem) in
@@ -258,7 +272,8 @@ val buffer_as_seq_reveal_tuint128
   [SMTPat (V.buffer128_as_seq va_s.VS.mem (as_vale_buffer x))]
 
 val immbuffer_as_seq_reveal_tuint128
-  (x:ibuf_t TUInt128)
+  (src:base_typ)
+  (x:ibuf_t src TUInt128)
   (va_s:V.va_state) : Lemma
   (let y = as_vale_immbuffer x in
    let h = hs_of_mem (as_mem va_s.VS.mem) in
@@ -267,6 +282,6 @@ val immbuffer_as_seq_reveal_tuint128
     (V.buffer128_as_seq va_s.VS.mem (as_vale_immbuffer x)))
   [SMTPat (V.buffer128_as_seq va_s.VS.mem (as_vale_immbuffer x))]
 
-val bounded_buffer_addrs (t:base_typ) (h:HS.mem) (b:buf_t t{B.live h b}) (s:ME.mem) : Lemma
-  (ME.buffer_addr #t (as_vale_buffer b) s + B.length b < Words_s.pow2_64)
+val bounded_buffer_addrs (src t:base_typ) (h:HS.mem) (b:buf_t src t{B.live h b}) (s:ME.mem) : Lemma
+  (ME.buffer_addr #t (as_vale_buffer b) s + DV.length (get_downview b) < Words_s.pow2_64)
 
